.

theories/System/Lambda1.v
@@ -39,6 +39,8 @@ Section STLC.
 
 #[local] Hint Resolve Name.ne_pirrel : core.
 
+#[local] Notation bty := (bty _).
+
 Context {L : language}.
 
 #[local] Notation typ := (typ L).
@@ -562,15 +564,15 @@ Proof.
   - econs 4.
 Defined.
 
-Fixpoint eval_typ (ty : typ) (Gamma : ctx) {struct ty} : Set :=
+Fixpoint eval_typ (Gamma : ctx) (ty : typ) {struct ty} : Set :=
   match ty with
-  | bty _ b => B.sig trm (fun u => typNe Gamma u (@bty L b))
-  | (ty1 -> ty2)%typ => forall Gamma' : ctx, le_ctx Gamma Gamma' -> eval_typ ty1 Gamma' -> eval_typ ty2 Gamma'
+  | bty b => B.sig trm (fun u => typNe Gamma u (bty b))
+  | (ty1 -> ty2)%typ => forall Gamma' : ctx, le_ctx Gamma Gamma' -> eval_typ Gamma' ty1 -> eval_typ Gamma' ty2
   end.
 
 Lemma le_ctx_preserves_eval_typ {Gamma} {ty}
-  (d : eval_typ ty Gamma)
-  : forall Delta : ctx, le_ctx Gamma Delta -> eval_typ ty Delta.
+  (d : eval_typ Gamma ty)
+  : forall Delta : ctx, le_ctx Gamma Delta -> eval_typ Delta ty.
 Proof.
   induction ty; simpl in *; intros Delta LE.
   - exists d.(B.proj1_sig). eapply le_ctx_preserves_typNe; [exact d.(B.proj2_sig) | exact LE].
@@ -579,8 +581,8 @@ Proof.
     + exact a.
 Defined.
 
-Fixpoint reflect (Gamma : ctx) (ty : typ) {struct ty} : B.sig trm (fun u => typNe Gamma u ty) -> eval_typ ty Gamma
-with reify (Gamma : ctx) (ty : typ) {struct ty} : eval_typ ty Gamma -> B.sig trm (fun v => typNf Gamma v ty).
+Fixpoint reflect (Gamma : ctx) (ty : typ) {struct ty} : B.sig trm (fun u => typNe Gamma u ty) -> eval_typ Gamma ty
+with reify (Gamma : ctx) (ty : typ) {struct ty} : eval_typ Gamma ty -> B.sig trm (fun v => typNf Gamma v ty).
 Proof.
   - destruct ty as [b | ty1 ty2]; simpl; intros u_hat.
     + eapply u_hat.
@@ -595,14 +597,14 @@ Proof.
       assert (y_hat : B.sig trm (fun u : trm => typNe ((y, ty1) :: Gamma) u ty1)).
       { exists (Var_trm y). econs 1. econs 1; reflexivity. }
       set (a := reflect ((y, ty1) :: Gamma) ty1 y_hat).
-      set (body := reify _ _ (d ((y, ty1) :: Gamma) claim1 a)).
+      set (body := reify ((y, ty1) :: Gamma) ty2 (d ((y, ty1) :: Gamma) claim1 a)).
       exists (Lam_trm y ty1 body.(B.proj1_sig)). econs 2. exact (body).(B.proj2_sig).
 Defined.
 
 Definition eval_ctx (Gamma : ctx) (Delta : ctx) : Set :=
-  forall x : name, forall ty : typ, Lookup x ty Gamma -> eval_typ ty Delta.
+  forall x : name, forall ty : typ, Lookup x ty Gamma -> eval_typ Delta ty.
 
-Fixpoint evalTyping Gamma e ty (TYPING : Typing Gamma e ty) {struct TYPING} : forall Delta : ctx, eval_ctx Gamma Delta -> eval_typ ty Delta.
+Fixpoint evalTyping Gamma e ty (TYPING : Typing Gamma e ty) {struct TYPING} : forall Delta : ctx, eval_ctx Gamma Delta -> eval_typ Delta ty.
 Proof.
   destruct TYPING; simpl; intros Delta rho.
   - refine (rho x ty LOOKUP).
@@ -610,12 +612,12 @@ Proof.
     intros x ty LOOKUP. exact LOOKUP.
   - intros Gamma' LE a.
     eapply evalTyping with (Gamma := (y, ty1) :: Gamma) (e := e1).
-    + exact TYPING.
-    + intros x ty LOOKUP. pattern LOOKUP. revert LOOKUP. eapply Lookup_cons.
-      * intros x_EQ ty_EQ. subst ty1. exact a.
-      * intros NE LOOKUP.
-        pose proof (rho_x := rho x ty LOOKUP).
-        exact (le_ctx_preserves_eval_typ rho_x Gamma' LE).
+    { exact TYPING. }
+    intros x ty LOOKUP. pattern LOOKUP. revert LOOKUP. eapply Lookup_cons.
+    + intros x_EQ ty_EQ. subst ty1. exact a.
+    + intros NE LOOKUP.
+      pose proof (rho_x := rho x ty LOOKUP).
+      exact (le_ctx_preserves_eval_typ rho_x Gamma' LE).
   - eapply reflect. exists (Con_trm c). econs 3. reflexivity.
 Defined.
 
