theories/System/STLC.v
@@ -19,7 +19,7 @@ Section STLC_META.
 
 Context {L : language}.
 
-Section KripkeLogicalRelation.
+Section Soundness_of_NbE.
 
 Context {Sigma : signature L}.
 
@@ -48,7 +48,26 @@ Proof.
   eapply SUBST_TYPING; exact LOOKUP.
 Defined.
 
-End KripkeLogicalRelation.
+Lemma substTyping_Typing {Gamma : ctx L} {e : trm L} {ty : typ L} {s : subst L} {Delta : ctx L}
+  (TYPING : Gamma ⊢ e ⦂ ty)
+  (SUBST_TYPING : substTyping Delta s Gamma)
+  : Delta ⊢ subst_trm s e ⦂ ty.
+Proof.
+Admitted.
+
+Fixpoint interpret_typ (Gamma : ctx L) (ty : typ L) {struct ty} : eval_typ Gamma ty -> trm L -> Prop :=
+  match ty as ty return eval_typ Gamma ty -> trm L -> Prop with
+  | bty _ b => fun d : B.sig (trm L) (fun u => typNe Gamma u (bty _ b)) => fun e : trm L =>
+    Gamma ⊢ d.(B.proj1_sig) = e ⦂ bty _ b
+  | (ty1 -> ty2)%typ => fun d : forall Gamma' : ctx L, le_ctx Gamma Gamma' -> eval_typ Gamma' ty1 -> eval_typ Gamma' ty2 => fun e1 : trm L =>
+    forall Gamma' : ctx L, forall LE : le_ctx Gamma Gamma', forall a : eval_typ Gamma' ty1, forall e2 : trm L, interpret_typ Gamma' ty1 a e2 -> interpret_typ Gamma' ty2 (d Gamma' LE a) (App_trm e1 e2)
+  end.
+
+Definition interpret_ctx (Gamma : ctx L) (Delta : ctx L) : eval_ctx Gamma Delta -> subst L -> Prop :=
+  fun rho : eval_ctx Gamma Delta => fun gamma : subst L =>
+  forall x : name, forall ty : typ L, forall LOOKUP : Lookup x ty Gamma, interpret_typ Delta ty (rho x ty LOOKUP) (gamma x).
+
+End Soundness_of_NbE.
 
 End STLC_META.
 
